dia24

CODIGO/GRAFOS/Auxiliar/Graph.dfy
@@ -5,15 +5,29 @@ type Graph = (set<Node>, set<Edge>)
 
 
 function invert (graph:Graph) : (r:Graph)
+requires isValidGraph(graph)
+ensures isValidGraph(r)
 {
     var allEdges:set<Edge> := (set n1,n2 | n1 in graph.0 && n2 in graph.0 && n1 != n2 :: {n1,n2});
     var invertGraph:Graph := (graph.0, allEdges-graph.1);
     (invertGraph)
 }
 
+
 predicate isValidGraph(graph: Graph)
 {
-    forall e | e in graph.1 :: (|e| == 2 && forall n | n in e :: n in graph.0)
+    forall e | e in graph.1 :: 
+    (|e| == 2 
+     && exists u,v :: u in graph.0 && v in graph.0 && u != v && e == {u,v} 
+    )
 }
+
+lemma intersect(s: set<Node>, graph:Graph, e: Edge)
+requires isValidGraph(graph)
+requires e in graph.1
+requires s <= graph.0
+ensures |s * e| <= 2 
+ensures var u,v :| u in graph.0 && v in graph.0 && u != v && e == {u,v}; 
+  s * e == {} || s * e == {u} || s * e == {v} || s * e == e 
 
 
