CODIGO/SUMA/Transformations/SumaNatToIntervalo.dfy
@@ -3,24 +3,24 @@ include "../Problems/SumaNat.dfy"
 include "../Problems/Intervalo.dfy"
 
 
-function Suma_to_Intervalo(A:multiset<nat>, S:nat) : (r:(multiset<nat>, nat, nat))
+function SumaNat_to_Intervalo(A:multiset<nat>, S:nat) : (r:(multiset<nat>, nat, nat))
 {
     (A, S, S+1)
 }
 
-lemma Suma_Intervalo(A:multiset<nat>, S:nat)
-  ensures var (IE,IS,IT) := Suma_to_Intervalo(A, S);
+lemma SumaNat_Intervalo(A:multiset<nat>, S:nat)
+  ensures var (IE,IS,IT) := SumaNat_to_Intervalo(A, S);
           SumaNat(A,S) <==> Intervalo(IE,IS,IT)
 { 
-    Suma_Intervalo1(A,S);
-    Suma_Intervalo2(A,S);
+    SumaNat_Intervalo1(A,S);
+    SumaNat_Intervalo2(A,S);
 }
 
-lemma Suma_Intervalo1(A:multiset<nat>, S:nat)
-    ensures var (IE,IS,IT) := Suma_to_Intervalo(A, S);
+lemma SumaNat_Intervalo1(A:multiset<nat>, S:nat)
+    ensures var (IE,IS,IT) := SumaNat_to_Intervalo(A, S);
           SumaNat(A,S) <== Intervalo(IE,IS,IT)
 {   
-    var (IE,IS,IT) := Suma_to_Intervalo(A,S);
+    var (IE,IS,IT) := SumaNat_to_Intervalo(A,S);
     // IE = {1, 2, 4}, IS = 6, IT = 7
     if (Intervalo(IE,IS,IT)) {
         var C:multiset<int> :| C <= IE && IS <= GSumNat(C) < IT; // C = 2, 4  ->  Sum(C) = 6
@@ -28,13 +28,13 @@ lemma Suma_Intervalo1(A:multiset<nat>, S:nat)
     }
 }
 
-lemma Suma_Intervalo2(A:multiset<nat>, S:nat)
-    ensures var (IE,IS,IT) := Suma_to_Intervalo(A,S);
+lemma SumaNat_Intervalo2(A:multiset<nat>, S:nat)
+    ensures var (IE,IS,IT) := SumaNat_to_Intervalo(A,S);
           SumaNat(A,S) ==> Intervalo(IE,IS,IT)
 {
     // A = {1, 2, 4}, S = 6
     if (SumaNat(A,S)) {
-        var (IE,IS,IT) := Suma_to_Intervalo(A,S);
+        var (IE,IS,IT) := SumaNat_to_Intervalo(A,S);
 
         var C:multiset<int> :| C <= A && GSumNat(C) == S; // C = 2, 4  ->  Sum(C) = 6
         assert S == IS <= GSumNat(C) < IT == S+1; // IS <= 6 < IT
