CODIGO/GRAFOS/Problems/Clique.dfy
@@ -1,12 +1,15 @@
 include "../Auxiliar/Graph.dfy"
 
 ghost predicate Clique(graph:Graph, k:int)
+requires isValidGraph(graph)
 {
-  exists s:set<Node> :: isClique(s,graph.1) && |s| >= k && s <= graph.0
+  exists s:set<Node> :: s <= graph.0 && isClique(s,graph) && |s| >= k 
 }
 
-ghost predicate isClique(s:set<Node>, E:set<set<Node>>)
+ghost predicate isClique(s:set<Node>, graph:Graph)
+requires isValidGraph(graph)
+requires s <= graph.0
 {
-  forall u,v | u in s && v in s && u != v :: {u,v} in E
+  forall u,v | u in s && v in s && u != v :: {u,v} in graph.1
 }
 
