CODIGO/GRAFOS/Problems/IndependentSet.dfy
@@ -1,35 +1,45 @@
 include "../Auxiliar/Graph.dfy"
 
 ghost predicate IndependentSet(graph:Graph, k:int)
+  requires isValidGraph(graph)
 {
-  exists s:set<Node> :: isIndependentSet(s,graph.1) && |s| >= k && s <= graph.0
+  exists s:set<Node> :: s <= graph.0 && isIndependentSet(s,graph) && |s| >= k 
 }
 
-ghost predicate isIndependentSet(s:set<Node>, E:set<Edge>)
+ghost predicate isIndependentSet(s:set<Node>, graph:Graph)
+requires isValidGraph(graph)
+requires  s <= graph.0
 {
-  forall e | e in E :: |s * e| <= 1
+  forall e | e in graph.1 :: |s * e| <= 1
 }
 
 lemma auxIndependentSet (IndepSet:set<Node>, graph:Graph)
-    ensures (forall e | e in graph.1 :: |IndepSet * e| <= 1) <==> (forall u,v | u in IndepSet && v in IndepSet && u != v :: {u,v} !in graph.1)
+    requires isValidGraph(graph) && IndepSet <= graph.0 
+    ensures isIndependentSet(IndepSet,graph) <==> (forall u,v | u in IndepSet && v in IndepSet && u != v :: {u,v} !in graph.1)
 {
   auxIndependentSet1(IndepSet,graph);
   auxIndependentSet2(IndepSet,graph);
 }
 
 lemma auxIndependentSet1 (IndepSet:set<Node>, graph:Graph)
-  ensures (forall e | e in graph.1 :: |IndepSet * e| <= 1) <== (forall u,v | u in IndepSet && v in IndepSet && u != v :: {u,v} !in graph.1)
+  requires isValidGraph(graph) && IndepSet <= graph.0
+  ensures isIndependentSet(IndepSet,graph) <== (forall u,v | u in IndepSet && v in IndepSet && u != v :: {u,v} !in graph.1)
 {
-  if (forall u,v | u in IndepSet && v in IndepSet && u != v :: {u,v} !in graph.1) {
-    
+  if (forall w,z | w in IndepSet && z in IndepSet && w != z :: {w,z} !in graph.1) {
+      assume exists e | e in graph.1 :: |IndepSet * e| > 1;
+      var e :| e in graph.1 && |IndepSet * e| > 1;
+      var u,v :| u in graph.0 && v in graph.0 && u !=v && e == {u,v};
+      intersect(IndepSet,graph,e);
 
-    assume forall e | e in graph.1 :: |IndepSet * e| <= 1;
+      assert u in IndepSet && v in IndepSet && u != v && {u,v} in graph.1;//La contradiccion
+      assert false;  
   }
 }
 
 
 lemma auxIndependentSet2 (IndepSet:set<Node>, graph:Graph)
-  ensures (forall e | e in graph.1 :: |IndepSet * e| <= 1) ==> (forall u,v | u in IndepSet && v in IndepSet && u != v :: {u,v} !in graph.1)
+  requires isValidGraph(graph) && IndepSet <= graph.0
+  ensures isIndependentSet(IndepSet,graph) ==> (forall u,v | u in IndepSet && v in IndepSet && u != v :: {u,v} !in graph.1)
 
 {
   if (forall e | e in graph.1 :: |IndepSet * e| <= 1) {
