CODIGO/GRAFOS/Problems/VertexCover.dfy
@@ -1,11 +1,14 @@
 include "../Auxiliar/Graph.dfy"
 
 ghost predicate VertexCover(graph:Graph, k:int)
+requires isValidGraph(graph)
 {
-  exists s:set<Node> :: isVertexCover(s,graph.1) && |s| <= k && s <= graph.0
+  exists s:set<Node> :: s <= graph.0 && isVertexCover(s,graph) && |s| <= k  
 }
 
-ghost predicate isVertexCover(s:set<Node>, E:set<set<Node>>)
+ghost predicate isVertexCover(s:set<Node>, graph:Graph)
+requires isValidGraph(graph)
+requires s <= graph.0
 {
-  forall e | e in E :: |s * e| > 0
+  forall e | e in graph.1 :: |s * e| > 0
 }
